

$$x = y^r - r \quad x = y$$

$$y = y^r - r \rightarrow y^r - y - r = 0$$

$$(y-r)(y+1) = 0 \quad \begin{cases} y=r \\ y=-1 \end{cases}$$

$$\int_{-1}^r \int_{y^r-r}^y dx dy = \int_{-1}^r (x) dy = \int_{-1}^r y - (y^r - r) dy$$

$$= \left(\frac{y^2}{2} - \frac{y^{r+1}}{r+1} + ry \right) \Big|_{-1}^r = \frac{r^2}{2} - \frac{r^{r+1}}{r+1} + r^2 - \left(\frac{1}{2} - \frac{1}{r+1} - r \right)$$

$$= \frac{r^2}{2} - \frac{r^{r+1}}{r+1} + r^2 - \frac{1}{2} + \frac{1}{r+1} + r = \frac{r^2}{2} - \frac{r^{r+1}}{r+1} + \frac{3r^2}{2} + \frac{1}{r+1}$$

$$y = \sin x \quad x = 0$$

$$y = x+1 \quad x = \frac{\pi}{2}$$

$$\int_0^{\frac{\pi}{2}} \int_{\sin x}^{x+1} dy dx = \int_0^{\frac{\pi}{2}} (y)_{\sin x}^{x+1} dx = \int_0^{\frac{\pi}{2}} (x+1) - \sin x dx$$

$$= \left(\frac{x^2}{2} + x + \cos x \right) \Big|_0^{\frac{\pi}{2}} = \frac{\frac{\pi^2}{4}}{2} + \frac{\pi}{2} + \cos \frac{\pi}{2} - \cos 0$$

$$= \frac{\pi^2}{8} + \frac{\pi}{2} + 0 - 1 = \frac{\pi^2}{8} + \frac{\pi}{2} - 1$$

$$\cos \rightarrow -\sin x$$

$$xy=1 \quad y=0 \quad x=\frac{1}{\varepsilon} \quad x=\varepsilon$$

$$y = \frac{1}{x}$$


$$\int_{\frac{1}{\varepsilon}}^{\varepsilon} \int_0^{\frac{1}{x}} dy dx = \int_{\frac{1}{\varepsilon}}^{\varepsilon} (y)_0^{\frac{1}{x}} dx = \int_{\frac{1}{\varepsilon}}^{\varepsilon} \frac{1}{x} dx = \left(\ln |x| \right)_{\frac{1}{\varepsilon}}^{\varepsilon} = \ln \varepsilon - \ln \frac{1}{\varepsilon}$$

$$= \ln \varepsilon + \ln \varepsilon = 2 \ln \varepsilon = \ln 14$$

$$\int_{\frac{1}{\varepsilon}}^{\varepsilon} \frac{1}{x} dx = 2 \ln \varepsilon$$


$x^2 + y^2 = \epsilon$ و $z = x^2 + y^2$ حاصل شده از تغییر در سطح
 $z = r^2$
 در سطح xy است، باید (r, θ, z)

$$\iint_R f \, dA = \int_0^{2\pi} \int_0^r f(r, \theta) r \, dr \, d\theta$$

$R: \begin{cases} 0 \leq r \leq r \\ 0 \leq \theta \leq 2\pi \end{cases}$


$$\int_0^{2\pi} \int_0^r \frac{r^n}{r^m} r \, dr \, d\theta = \int_0^{2\pi} \left(\frac{r^n}{r^m} \right) d\theta = \int_0^{2\pi} r \, d\theta = (r\theta) \Big|_0^{2\pi} = 2\pi r$$

$xy = 1$ $y = 0$ $x = \frac{1}{\epsilon}$ $x = \frac{1}{\epsilon}$
 $y = \frac{1}{x}$


 $\int_{\frac{1}{\epsilon}}^{\epsilon} \int_0^{\frac{1}{x}} dy \, dx = \int_{\frac{1}{\epsilon}}^{\epsilon} (y) \Big|_0^{\frac{1}{x}} dx = \int_{\frac{1}{\epsilon}}^{\epsilon} \frac{1}{x} dx = (\ln |x|) \Big|_{\frac{1}{\epsilon}}^{\epsilon} = \ln \epsilon - \ln \frac{1}{\epsilon}$
 $= \ln \epsilon + \ln \epsilon = 2 \ln \epsilon = \ln \epsilon^2$

$$\log_c a + \log_c b = \log_c ab$$

$$\log_c a^n = \log_c a \cdot a \cdot a \dots a = \log_c a + \log_c a + \dots + \log_c a = n \log_c a$$

$$1) f(x, y) = \begin{cases} \frac{x^r - y^r}{x + y} \\ \infty \end{cases}$$

$$(x, y) \neq (1, -1) \\ (x, y) = (1, -1)$$

$$f(x, y) = \frac{x^r + y^r}{x - y} \quad (-1, 1)$$

$$f_{(1,1)} = \infty$$

$$\lim_{(x,y) \rightarrow (1,-1)} f = \frac{x^r - y^r}{x + y} = \frac{(x+y)(x-y)}{x+y} = 1 - (-1) = 2$$

$$\lim_{(x,y) \rightarrow (1,1)} \frac{(x+y)(x^r - xy + y^r)}{(x-y)(x+y)} = \lim_{(x,y) \rightarrow (1,1)} \frac{x^r - xy + y^r}{(x-y)} = 2$$

$$\frac{(-1)^r - (-1)(1) + (1)^r}{-1-1} = \frac{1+1+1}{-2} = -\frac{3}{2}$$

$$\cos u = -u' \sin u$$

$$1) w = \cos y - \sin z \rightarrow dw = -\sin y dy + (-\sin y dy) - \cos z dz$$

$$2) z = x^r + x^r y^r - y^r \rightarrow dz = (r x^{r-1} + r x^r y^{r-1}) dx + (r y x^{r-1} - r y^{r-1}) dy$$

$$f(x, y) \frac{x^r + y^r}{x^r - y^r} \quad (-1, 1)$$

$$\lim_{(x, y) \rightarrow (-1, 1)} \frac{(x+y)(x^r - xy + y^r)}{(x-y)(x+y)} = \lim_{(x, y) \rightarrow (-1, 1)} \frac{x^r - xy + y^r}{(x-y)} = 2$$

$$\frac{(-1)^r - (-1)(1) + (1)^r}{-1-1} = \frac{1+1+1}{-2} = -\frac{3}{2}$$

$$3. f(x, y, z) = x^2 + y^2 - z^2 \quad P(1, 1, 1) \quad V = -x\vec{i} + y\vec{j} + z\vec{k}$$

$$|\vec{V}| = \sqrt{(-1)^2 + 1^2 + 1^2} = \sqrt{3} = V$$

$$\vec{u}_n = \frac{1}{V} (-x\vec{i} + y\vec{j} + z\vec{k}) = \frac{-1}{\sqrt{3}}\vec{i} + \frac{1}{\sqrt{3}}\vec{j} + \frac{1}{\sqrt{3}}\vec{k}$$

$$f_x = 2x \quad f_x = (1, 1, 1) = 2$$

$$f_y = 2y \quad f_y = (1, 1, 1) = 2$$

$$f_z = -2z \quad f_z = (1, 1, 1) = -2$$

$$D_u f = -1 \times \frac{1}{\sqrt{3}} + 1 \times \frac{1}{\sqrt{3}} + (-2 \times \frac{1}{\sqrt{3}}) = \frac{-1}{\sqrt{3}} + \frac{1}{\sqrt{3}} - \frac{2}{\sqrt{3}} = \frac{-2}{\sqrt{3}}$$